

$$1) \quad T(z_{in}) = \frac{1}{1 + e^{-2z_{in}}} = \sigma(2z_{in})$$

$$\hookrightarrow T(z_{in}) = \sigma(2 \cdot (\omega^T x + b))$$

To match the second neuron with the first we need:

$$T(z_{in}) = x'_{out} = \sigma(\omega'^T x + b')$$

Now we can say:

$$\sigma(\omega'^T x + b') = \sigma(2 \cdot (\omega^T x + b))$$

We can match the inside because sigmoid is strictly increasing, therefore if  $\sigma(a) = \sigma(b)$  then  $a = b$ .

$$\omega'^T x + b' = 2(\omega^T x + b)$$

$$\omega'^T x + b' = 2\omega^T x + 2b$$

$$\hookrightarrow \omega' = 2\omega \quad b' = 2b$$

2

 $g = \text{ReLU}$ 

$$2) f_{in} = U \cdot g(Wx + b) + c$$

$$Wx = \begin{pmatrix} 1 & 1 \\ 1 & 1 \end{pmatrix} \cdot \begin{pmatrix} 0 & 0 \\ 0 & 1 \\ 1 & 0 \\ 1 & 1 \end{pmatrix} = \begin{pmatrix} 0 & 0 \\ 1 & 1 \\ 1 & 1 \\ 2 & 2 \end{pmatrix}$$

$$Wx + b = \begin{pmatrix} 0 & 0 \\ 1 & 1 \\ 1 & 1 \\ 2 & 2 \end{pmatrix} + \begin{pmatrix} 0 \\ -1 \end{pmatrix} = \begin{pmatrix} 0 & -1 \\ 1 & 0 \\ 1 & 0 \\ 2 & 1 \end{pmatrix} = z$$

$$\text{ReLU}(z) = \begin{pmatrix} 0 & 0 \\ 1 & 0 \\ 1 & 0 \\ 2 & 1 \end{pmatrix} = z_R$$

$$U \cdot z_R = \begin{pmatrix} 0 & 0 \\ 1 & 0 \\ 1 & 0 \\ 2 & 1 \end{pmatrix} \cdot \begin{pmatrix} 1 \\ -2 \end{pmatrix} = \begin{pmatrix} 0 \\ 1 \\ 1 \\ 0 \end{pmatrix} = z_{zu}$$

$$z_{zu} + c = \begin{pmatrix} 0 \\ 1 \\ 1 \\ 0 \end{pmatrix} + (-0.5) = \begin{pmatrix} -0.5 \\ 0.5 \\ 0.5 \\ -0.5 \end{pmatrix} = f_{in}$$

$J(f_{in})$  will return the expected results for XOR modelling.

b) change  $u$  to  $\begin{pmatrix} 1 \\ -1 \end{pmatrix}$  to model OR and change  $u$  to  $\begin{pmatrix} 0 \\ 1 \end{pmatrix}$  to model AND.  $c$  can stay  $-0,5$  for both scenarios.